src/Lean/Elab/Tactic/Grind/BuiltinTactic.lean
@@ -12,6 +12,9 @@ import Lean.Meta.Tactic.Grind.Arith.Cutsat.Search
 import Lean.Meta.Tactic.Grind.Arith.CommRing.EqCnstr
 import Lean.Meta.Tactic.Grind.EMatch
 import Lean.Meta.Tactic.Grind.Intro
+import Lean.Meta.Tactic.Grind.Split
+import Lean.Meta.Tactic.Grind.Anchor
+import Lean.Elab.Tactic.Basic
 namespace Lean.Elab.Tactic.Grind
 
 def evalSepTactics (stx : Syntax) : GrindTacticM Unit := do
@@ -77,5 +80,109 @@ open Meta Grind
     discard <| assertAll
     getGoal
   replaceMainGoal [goal]
+
+@[builtin_grind_tactic cases] def evalCases : GrindTactic := fun stx => do
+  match stx with
+  | `(grind| cases #$anchor:hexnum) =>
+    let numDigits := anchor.getHexNumSize
+    let val := anchor.getHexNumVal
+    if val >= UInt64.size then
+      throwError "invalid anchor, value is too big"
+    let val := val.toUInt64
+    let goal ← getMainGoal
+    let candidates := goal.split.candidates
+    let (goals, genNew) ← liftSearchM do
+      for c in candidates do
+        let anchor ← getAnchor c.getExpr
+        if isAnchorPrefix numDigits val anchor then
+          let some result ← split? c
+            | throwError "`cases` tactic failed, case-split is not ready{indentExpr c.getExpr}"
+          return result
+      throwError "`cases` tactic failed, invalid anchor"
+    let goals ← goals.filterMapM fun goal => do
+      let (goal, _) ← liftGrindM <| SearchM.run goal do
+        intros genNew
+        getGoal
+      if goal.inconsistent then
+        return none
+      else
+        return some goal
+    replaceMainGoal goals
+  | _ => throwUnsupportedSyntax
+
+@[builtin_grind_tactic Parser.Tactic.Grind.focus] def evalFocus : GrindTactic := fun stx => do
+  let mkInfo ← mkInitialTacticInfo stx[0]
+  focus do
+    -- show focused state on `focus`
+    withInfoContext (pure ()) mkInfo
+    evalGrindTactic stx[1]
+
+@[builtin_grind_tactic allGoals] def evalAllGoals : GrindTactic := fun stx => do
+  let goals ← getGoals
+  let mut goalsNew := #[]
+  let mut abort := false
+  for goal in goals do
+    unless (← goal.mvarId.isAssigned) do
+      setGoals [goal]
+      let saved ← saveState
+      abort ← Grind.tryCatch
+        (do
+          evalGrindTactic stx[1]
+          pure abort)
+        (fun ex => do
+          if (← read).recover then
+            logException ex
+            let msgLog ← Core.getMessageLog
+            saved.restore
+            Core.setMessageLog msgLog
+            admitGoal goal.mvarId
+            pure true
+          else
+            throw ex)
+      goalsNew := goalsNew ++ (← getUnsolvedGoals)
+  if abort then
+    throwAbortTactic
+  setGoals goalsNew.toList
+
+@[builtin_grind_tactic withAnnotateState] def evalWithAnnotateState : GrindTactic := fun stx =>
+  withTacticInfoContext stx[1] do
+  evalGrindTactic stx[2]
+
+@[builtin_grind_tactic anyGoals] def evalAnyGoals : GrindTactic := fun stx => do
+  let goals ← getGoals
+  let mut goalsNew := #[]
+  let mut succeeded := false
+  for goal in goals do
+    unless (← goal.mvarId.isAssigned) do
+      setGoals [goal]
+      try
+        evalGrindTactic stx[1]
+        goalsNew := goalsNew ++ (← getUnsolvedGoals)
+        succeeded := true
+      catch _ =>
+        goalsNew := goalsNew.push goal
+  unless succeeded do
+    throwError "Tactic failed on all goals:{indentD stx[1]}"
+  setGoals goalsNew.toList
+
+@[builtin_grind_tactic «next»] def evalNext : GrindTactic := fun stx => do
+  match stx with
+  | `(grind| next%$nextTk =>%$arr $seq:grindSeq) => do
+    let goal :: goals ← getUnsolvedGoals | throwNoGoalsToBeSolved
+    setGoals [goal]
+    goal.mvarId.setTag Name.anonymous
+    withCaseRef arr seq <| closeUsingOrAdmit <| withTacticInfoContext (mkNullNode #[nextTk, arr]) <|
+      evalGrindTactic stx[2]
+    setGoals goals
+  | _ => throwUnsupportedSyntax
+
+@[builtin_grind_tactic nestedTacticCore] def evalNestedTactic : GrindTactic := fun stx => do
+  match stx with
+  | `(grind| tactic%$tacticTk =>%$arr $seq:tacticSeq) => do
+    let goal ← getMainGoal
+    discard <| Tactic.run goal.mvarId <| withCaseRef arr seq <| Tactic.closeUsingOrAdmit
+      <| Tactic.withTacticInfoContext (mkNullNode #[tacticTk, arr]) <| evalTactic seq
+    replaceMainGoal []
+  | _ => throwUnsupportedSyntax
 
 end Lean.Elab.Tactic.Grind
